src/Spec/Compile.v
@@ -381,21 +381,8 @@ Section Atomization.
     - eapply trace_incl_bind_a; eauto.
     - repeat rewrite exec_equiv_bind_bind.
       eauto.
-    - etransitivity.
-      eapply trace_incl_rx_to_trace_incl.
-      eapply trace_incl_rx_until.
-      intros. eapply trace_incl_to_trace_incl_rx; intros.
-      eapply H0; intros.
-      reflexivity.
-      eapply trace_incl_bind_a; intros.
-      eauto.
-    - etransitivity.
-      eapply trace_incl_rx_to_trace_incl.
-      eapply trace_incl_rx_spawn.
-      eapply trace_incl_to_trace_incl_rx; intros.
-      eapply IHatomize_ok; reflexivity.
-      eapply trace_incl_bind_a; intros.
-      eauto.
+    - eapply trace_incl_rx'_until; eauto.
+    - eapply trace_incl_rx'_spawn; eauto.
   Qed.
 
   Theorem atomize_ok_trace_incl :
